Steel.Memory: Rename mem -> heap and t -> mem

pulse/ulib/experimental/Steel.Memory.fst
@@ -32,21 +32,21 @@ let addr = nat
 /// This is just the core of a memory, about which one can write
 /// assertions. At one level above, we'll encapsulate this memory
 /// with a freshness counter, a lock store etc.
-let mem = addr ^-> option cell
+let heap = addr ^-> option cell
 
-let contains_addr (m:mem) (a:addr)
+let contains_addr (m:heap) (a:addr)
   : bool
   = Some? (m a)
 
-let select_addr (m:mem) (a:addr{contains_addr m a})
+let select_addr (m:heap) (a:addr{contains_addr m a})
   : cell
   = Some?.v (m a)
 
-let update_addr (m:mem) (a:addr) (c:cell)
-  : mem
+let update_addr (m:heap) (a:addr) (c:cell)
+  : heap
   = F.on _ (fun a' -> if a = a' then Some c else m a')
 
-let disjoint_addr (m0 m1:mem) (a:addr)
+let disjoint_addr (m0 m1:heap) (a:addr)
   : prop
   = match m0 a, m1 a with
     | Some (Ref t0 p0 v0), Some (Ref t1 p1 v1) ->
@@ -64,16 +64,16 @@ let disjoint_addr (m0 m1:mem) (a:addr)
 
 let ref (a:Type) = addr
 
-let disjoint (m0 m1:mem)
+let disjoint (m0 m1:heap)
   : prop
   = forall a. disjoint_addr m0 m1 a
 
-let disjoint_sym (m0 m1:mem)
+let disjoint_sym (m0 m1:heap)
   : Lemma (disjoint m0 m1 <==> disjoint m1 m0)
   = ()
 
-let join (m0:mem) (m1:mem{disjoint m0 m1})
-  : mem
+let join (m0:heap) (m1:heap{disjoint m0 m1})
+  : heap
   = F.on _ (fun a ->
       match m0 a, m1 a with
       | None, None -> None
@@ -82,7 +82,7 @@ let join (m0:mem) (m1:mem{disjoint m0 m1})
       | Some (Ref a0 p0 v0), Some (Ref a1 p1 v1) ->
         Some (Ref a0 (p0 +. p1) v0))
 
-let disjoint_join' (m0 m1 m2:mem)
+let disjoint_join' (m0 m1 m2:heap)
   : Lemma (disjoint m1 m2 /\
            disjoint m0 (join m1 m2) ==>
            disjoint m0 m1 /\
@@ -94,10 +94,10 @@ let disjoint_join' (m0 m1 m2:mem)
 
 let disjoint_join m0 m1 m2 = disjoint_join' m0 m1 m2
 
-let mem_equiv (m0 m1:mem) =
+let mem_equiv (m0 m1:heap) =
   forall a. m0 a == m1 a
 
-let mem_equiv_eq (m0 m1:mem)
+let mem_equiv_eq (m0 m1:heap)
   : Lemma
     (requires
       m0 `mem_equiv` m1)
@@ -106,7 +106,7 @@ let mem_equiv_eq (m0 m1:mem)
     [SMTPat (m0 `mem_equiv` m1)]
   = F.extensionality _ _ m0 m1
 
-let join_commutative' (m0 m1:mem)
+let join_commutative' (m0 m1:heap)
   : Lemma
     (requires
       disjoint m0 m1)
@@ -117,7 +117,7 @@ let join_commutative' (m0 m1:mem)
 
 let join_commutative m0 m1 = ()
 
-let join_associative' (m0 m1 m2:mem)
+let join_associative' (m0 m1 m2:heap)
   : Lemma
     (requires
       disjoint m1 m2 /\
@@ -130,9 +130,9 @@ let join_associative' (m0 m1 m2:mem)
        [SMTPat (join (join m0 m1) m2)]]]
   = ()
 
-let join_associative (m0 m1 m2:mem) = join_associative' m0 m1 m2
+let join_associative (m0 m1 m2:heap) = join_associative' m0 m1 m2
 
-let join_associative2 (m0 m1 m2:mem)
+let join_associative2 (m0 m1 m2:heap)
   : Lemma
     (requires
       disjoint m0 m1 /\
@@ -159,7 +159,7 @@ type hprop : Type u#1 =
   | Ex   : #a:Type0 -> (a -> hprop) -> hprop
   | All  : #a:Type0 -> (a -> hprop) -> hprop
 
-let rec interp (p:hprop) (m:mem)
+let rec interp (p:hprop) (m:heap)
   : Tot prop (decreases p)
   = match p with
     | Emp -> True
@@ -214,43 +214,43 @@ let star_associative (p1 p2 p3:hprop) = ()
 
 let star_congruence (p1 p2 p3 p4:hprop) = ()
 
-let sel #a (r:ref a) (m:hmem (ptr r))
+let sel #a (r:ref a) (m:hheap (ptr r))
   : a
   = let Ref _ _ v = select_addr m r in
     v
 
-let sel_lemma #a (r:ref a) (p:perm) (m:hmem (ptr_perm r p))
+let sel_lemma #a (r:ref a) (p:perm) (m:hheap (ptr_perm r p))
   = ()
 
 /// The main caveat of this model is that because we're working
 /// with proof-irrelevant propositions (squashed proofs), I end up
 /// using the indefinite_description axiom to extract witnesses
 /// of disjoint memories from squashed proofs of `star`
-let split_mem_ghost (p1 p2:hprop) (m:hmem (p1 `Star` p2))
-  : GTot (ms:(hmem p1 & hmem p2){
+let split_mem_ghost (p1 p2:hprop) (m:hheap (p1 `Star` p2))
+  : GTot (ms:(hheap p1 & hheap p2){
             let m1, m2 = ms in
             disjoint m1 m2 /\
             m == join m1 m2})
   = let open FStar.IndefiniteDescription in
     let (| m1, p |)
-      : (m1:mem &
-        (exists (m2:mem).
+      : (m1:heap &
+        (exists (m2:heap).
           m1 `disjoint` m2 /\
           m == join m1 m2 /\
           interp p1 m1 /\
           interp p2 m2))
         =
       indefinite_description
-        mem
-        (fun (m1:mem) ->
-          exists (m2:mem).
+        heap
+        (fun (m1:heap) ->
+          exists (m2:heap).
             m1 `disjoint` m2 /\
             m == join m1 m2 /\
             interp p1 m1 /\
             interp p2 m2)
     in
     let p :
-      (exists (m2:mem).
+      (exists (m2:heap).
         m1 `disjoint` m2 /\
         m == join m1 m2 /\
         interp p1 m1 /\
@@ -259,8 +259,8 @@ let split_mem_ghost (p1 p2:hprop) (m:hmem (p1 `Star` p2))
     let _ = FStar.Squash.return_squash p in
     let (| m2, _ |) =
       indefinite_description
-        mem
-        (fun (m2:mem) ->
+        heap
+        (fun (m2:heap) ->
            m1 `disjoint` m2 /\
            m == join m1 m2 /\
            interp p1 m1 /\
@@ -282,16 +282,16 @@ assume
 val axiom_ghost_to_tot (#a:Type) (#b:a -> Type) ($f: (x:a -> GTot (b x))) (x:a)
   : Tot (b x)
 
-let split_mem (p1 p2:hprop) (m:hmem (p1 `Star` p2))
-  : Tot (ms:(hmem p1 & hmem p2){
+let split_mem (p1 p2:hprop) (m:hheap (p1 `Star` p2))
+  : Tot (ms:(hheap p1 & hheap p2){
             let m1, m2 = ms in
             disjoint m1 m2 /\
             m == join m1 m2})
   = axiom_ghost_to_tot (split_mem_ghost p1 p2) m
 
 let upd #a (r:ref a) (v:a)
-           (frame:hprop) (m:hmem (ptr_perm r 1.0R  `Star` frame))
-  : Tot (m:hmem (Pts_to r 1.0R v `Star` frame))
+           (frame:hprop) (m:hheap (ptr_perm r 1.0R  `Star` frame))
+  : Tot (m:hheap (Pts_to r 1.0R v `Star` frame))
   = let m0, m1 = split_mem (ptr_perm r 1.0R) frame m in
     let m0' = update_addr m0 r (Ref a 1.0R v) in
     join m0' m1
@@ -299,23 +299,23 @@ let upd #a (r:ref a) (v:a)
 ////////////////////////////////////////////////////////////////////////////////
 // wand
 ////////////////////////////////////////////////////////////////////////////////
-let intro_wand_alt (p1 p2:hprop) (m:mem)
+let intro_wand_alt (p1 p2:hprop) (m:heap)
   : Lemma
     (requires
-      (forall (m0:hmem p1).
+      (forall (m0:hheap p1).
          disjoint m0 m ==>
          interp p2 (join m0 m)))
     (ensures
       interp (wand p1 p2) m)
   = ()
 
-let intro_wand (p q r:hprop) (m:hmem q)
+let intro_wand (p q r:hprop) (m:hheap q)
   : Lemma
     (requires
-      (forall (m:hmem (p `star` q)). interp r m))
+      (forall (m:hheap (p `star` q)). interp r m))
     (ensures
       interp (p `wand` r) m)
-  = let aux (m0:hmem p)
+  = let aux (m0:hheap p)
       : Lemma
         (requires
           disjoint m0 m)
@@ -326,27 +326,27 @@ let intro_wand (p q r:hprop) (m:hmem q)
     in
     intro_wand_alt p r m
 
-let elim_wand (p1 p2:hprop) (m:mem) = ()
+let elim_wand (p1 p2:hprop) (m:heap) = ()
 
 ////////////////////////////////////////////////////////////////////////////////
 // or
 ////////////////////////////////////////////////////////////////////////////////
 
-let intro_or_l (p1 p2:hprop) (m:hmem p1)
+let intro_or_l (p1 p2:hprop) (m:hheap p1)
   : Lemma (interp (h_or p1 p2) m)
   = ()
 
-let intro_or_r (p1 p2:hprop) (m:hmem p2)
+let intro_or_r (p1 p2:hprop) (m:hheap p2)
   : Lemma (interp (h_or p1 p2) m)
   = ()
 
-let or_star (p1 p2 p:hprop) (m:hmem ((p1 `star` p) `h_or` (p2 `star` p)))
+let or_star (p1 p2 p:hprop) (m:hheap ((p1 `star` p) `h_or` (p2 `star` p)))
   : Lemma (interp ((p1 `h_or` p2) `star` p) m)
   = ()
 
-let elim_or (p1 p2 q:hprop) (m:hmem (p1 `h_or` p2))
-  : Lemma (((forall (m:hmem p1). interp q m) /\
-            (forall (m:hmem p2). interp q m)) ==> interp q m)
+let elim_or (p1 p2 q:hprop) (m:hheap (p1 `h_or` p2))
+  : Lemma (((forall (m:hheap p1). interp q m) /\
+            (forall (m:hheap p2). interp q m)) ==> interp q m)
   = ()
 
 
@@ -354,13 +354,13 @@ let elim_or (p1 p2 q:hprop) (m:hmem (p1 `h_or` p2))
 // and
 ////////////////////////////////////////////////////////////////////////////////
 
-let intro_and (p1 p2:hprop) (m:mem)
+let intro_and (p1 p2:hprop) (m:heap)
   : Lemma (interp p1 m /\
            interp p2 m ==>
            interp (p1 `h_and` p2) m)
   = ()
 
-let elim_and (p1 p2:hprop) (m:hmem (p1 `h_and` p2))
+let elim_and (p1 p2:hprop) (m:hheap (p1 `h_and` p2))
   : Lemma (interp p1 m /\
            interp p2 m)
   = ()
@@ -370,11 +370,11 @@ let elim_and (p1 p2:hprop) (m:hmem (p1 `h_and` p2))
 // h_exists
 ////////////////////////////////////////////////////////////////////////////////
 
-let intro_exists (#a:_) (x:a) (p : a -> hprop) (m:hmem (p x))
+let intro_exists (#a:_) (x:a) (p : a -> hprop) (m:hheap (p x))
   : Lemma (interp (h_exists p) m)
   = ()
 
-let elim_exists (#a:_) (p:a -> hprop) (q:hprop) (m:hmem (h_exists p))
+let elim_exists (#a:_) (p:a -> hprop) (q:hprop) (m:hheap (h_exists p))
   : Lemma
     ((forall (x:a). interp (p x) m ==> interp q m) ==>
      interp q m)
@@ -385,17 +385,17 @@ let elim_exists (#a:_) (p:a -> hprop) (q:hprop) (m:hmem (h_exists p))
 // h_forall
 ////////////////////////////////////////////////////////////////////////////////
 
-let intro_forall (#a:_) (p : a -> hprop) (m:mem)
+let intro_forall (#a:_) (p : a -> hprop) (m:heap)
   : Lemma ((forall x. interp (p x) m) ==> interp (h_forall p) m)
   = ()
 
-let elim_forall (#a:_) (p : a -> hprop) (m:hmem (h_forall p))
+let elim_forall (#a:_) (p : a -> hprop) (m:hheap (h_forall p))
   : Lemma ((forall x. interp (p x) m) ==> interp (h_forall p) m)
   = ()
 
 ////////////////////////////////////////////////////////////////////////////////
 
-let intro_pts_to (#a:_) (x:ref a) (p:perm) (v:a) (m:mem)
+let intro_pts_to (#a:_) (x:ref a) (p:perm) (v:a) (m:heap)
   : Lemma
     (requires
        m `contains_addr` x /\
@@ -407,7 +407,7 @@ let intro_pts_to (#a:_) (x:ref a) (p:perm) (v:a) (m:mem)
        interp (pts_to x p v) m)
   = ()
 
-let intro_star (p q:hprop) (mp:hmem p) (mq:hmem q)
+let intro_star (p q:hprop) (mp:hheap p) (mq:hheap q)
   : Lemma
     (requires
       disjoint mp mq)
@@ -416,7 +416,7 @@ let intro_star (p q:hprop) (mp:hmem p) (mq:hmem q)
   = ()
 
 #push-options "--z3rlimit_factor 4 --max_fuel 2 --max_ifuel 2  --initial_fuel 2 --initial_ifuel 2"
-let rec affine_star_aux (p:hprop) (m:mem) (m':mem { disjoint m m' })
+let rec affine_star_aux (p:hprop) (m:heap) (m':heap { disjoint m m' })
   : Lemma
     (ensures interp p m ==> interp p (join m m'))
     [SMTPat (interp p (join m m'))]
@@ -430,7 +430,7 @@ let rec affine_star_aux (p:hprop) (m:mem) (m':mem { disjoint m m' })
     | Or p1 p2 -> affine_star_aux p1 m m'; affine_star_aux p2 m m'
 
     | Star p1 p2 ->
-      let aux (m1 m2:mem) (m':mem {disjoint m m'})
+      let aux (m1 m2:heap) (m':heap {disjoint m m'})
         : Lemma
           (requires
             disjoint m1 m2 /\
@@ -450,7 +450,7 @@ let rec affine_star_aux (p:hprop) (m:mem) (m':mem { disjoint m m' })
       ()
 
     | Wand p q ->
-      let aux (mp:hmem p)
+      let aux (mp:hheap p)
         : Lemma
           (requires
             disjoint mp (join m m') /\
@@ -484,7 +484,7 @@ let rec affine_star_aux (p:hprop) (m:mem) (m':mem { disjoint m m' })
       ()
 #pop-options
 
-let affine_star (p q:hprop) (m:mem)
+let affine_star (p q:hprop) (m:heap)
   : Lemma
     (ensures (interp (p `star` q) m ==> interp p m))
   = ()
@@ -493,25 +493,25 @@ let affine_star (p q:hprop) (m:mem)
 // emp
 ////////////////////////////////////////////////////////////////////////////////
 
-let intro_emp (m:mem)
+let intro_emp (m:heap)
   : Lemma (interp emp m)
   = ()
 
 let emp_unit (p:hprop)
   : Lemma
     ((p `star` emp) `equiv` p)
-  = let emp_unit_1 (p:hprop) (m:mem)
+  = let emp_unit_1 (p:hprop) (m:heap)
       : Lemma
         (requires interp p m)
         (ensures  interp (p `star` emp) m)
         [SMTPat (interp (p `star` emp) m)]
-      = let emp_m : mem = F.on _ (fun _ -> None) in
+      = let emp_m : heap = F.on _ (fun _ -> None) in
         assert (disjoint emp_m m);
         assert (interp (p `star` emp) (join m emp_m));
         assert (mem_equiv m (join m emp_m));
         intro_star p emp m emp_m
     in
-    let emp_unit_2 (p:hprop) (m:mem)
+    let emp_unit_2 (p:hprop) (m:heap)
       : Lemma
         (requires interp (p `star` emp) m)
         (ensures interp p m)
@@ -522,32 +522,32 @@ let emp_unit (p:hprop)
 
 ////////////////////////////////////////////////////////////////////////////////
 noeq
-type t = {
+type mem = {
   ctr: nat;
-  mem: mem;
+  heap: heap;
   properties: squash (
-    forall i. i >= ctr ==> mem i == None
+    forall i. i >= ctr ==> heap i == None
   )
 }
 
-let mem_of_t (x:t) : mem = x.mem
+let heap_of_mem (x:mem) : heap = x.heap
 
 let alloc #a v frame m
   = let x : ref a = m.ctr in
     let cell = Ref a 1.0R v in
-    let mem : mem = F.on _ (fun i -> if i = x then Some cell else None) in
-    assert (disjoint mem m.mem);
+    let mem : heap = F.on _ (fun i -> if i = x then Some cell else None) in
+    assert (disjoint mem m.heap);
     assert (mem `contains_addr` x);
     assert (select_addr mem x == cell);
-    let mem' = join mem m.mem in
+    let mem' = join mem m.heap in
     intro_pts_to x 1.0R v mem;
     assert (interp (pts_to x 1.0R v) mem);
-    assert (interp frame m.mem);
-    intro_star (pts_to x 1.0R v) frame mem m.mem;
+    assert (interp frame m.heap);
+    intro_star (pts_to x 1.0R v) frame mem m.heap;
     assert (interp (pts_to x 1.0R v `star` frame) mem');
     let t = {
       ctr = x + 1;
-      mem = mem';
+      heap = mem';
       properties = ()
     } in
     (| x, t |)
